Propagated the labelled transitions to the manually modified model and the monadic proofs.

mcontests.v
@@ -5,11 +5,11 @@ Require Import List.
 Load mconbase2.
 
 (*Check E_ident(0).*)
-Check JO_red (E_ident(0)) (E_ident(1)).
+Check JO_red (E_ident(0)) S_First RL_tau (E_ident(1)).
 
 
 Notation "A >>= F" := (E_bind A F) (at level 42, left associativity).
-Notation "A --> B" := (JO_red A B) (at level 54, no associativity).
+Notation "A [ C ] --> [ D ] B" := (JO_red A C D B) (at level 54, no associativity).
 
 
 Example valuepair : is_value_of_expr (E_pair (E_constant(CONST_ret)) (E_constant(CONST_fork))).
@@ -22,8 +22,8 @@ Ltac caseEq f :=
   generalize (refl_equal f); pattern f at -1; case f. 
 
 Inductive JO_red_star : expr -> expr -> Prop :=
-| JO_red_star_step: forall (e e' f : expr),
-    e --> e' ->
+| JO_red_star_step: forall (e e' f : expr) (s : select) (rl : redlabel),
+    e [ s ] --> [ rl ] e' ->
     JO_red_star e' f ->
     JO_red_star e f
 | JO_red_star_refl: forall e,
@@ -44,57 +44,57 @@ Qed.
 
 *)
 
-Lemma mon_left_id : forall (x:value_name) (t : typexpr) (a e:expr),
+Lemma mon_left_id : forall (x:value_name) (t : typexpr) (a e:expr) (s s' : select),
     is_value_of_expr a ->
     ((E_apply(E_constant (CONST_ret)) a) >>= (E_function x t e)) -->* (E_apply (E_function x t e) a).
 Proof.
  intros.
- apply JO_red_star_step with (e' := (E_live_expr a >>= E_function x t e)).
+ apply JO_red_star_step with (e' := (E_live_expr (LM_expr a) >>= E_function x t e))(s:=s)(rl:=RL_tau).
  apply JO_red_evalbind.
  apply JO_red_ret.
  apply H.
- apply JO_red_star_step with (e' := (E_apply (E_function x t e) a)).
+ apply JO_red_star_step with (e' := (E_apply (E_function x t e) a))(s:=s')(rl:=RL_tau).
  apply JO_red_dobind.
  apply H.
  apply JO_red_star_refl.
 Qed.
 
 
-Lemma mon_right_id : forall (a:expr),
+Lemma mon_right_id : forall (a:expr) (s s' : select),
    is_value_of_expr a ->
-   E_live_expr a >>= E_constant CONST_ret -->* E_live_expr a.
+   E_live_expr (LM_expr a) >>= E_constant CONST_ret -->* E_live_expr (LM_expr a).
 Proof.
  intros.
- apply JO_red_star_step with (e' := (E_apply (E_constant CONST_ret) a)).
+ apply JO_red_star_step with (e' := (E_apply (E_constant CONST_ret) a))(s:= s)(rl:=RL_tau).
  apply JO_red_dobind.
  trivial.
- apply JO_red_star_step with (e' := (E_live_expr a)).
+ apply JO_red_star_step with (e' := (E_live_expr (LM_expr a)))(s:=s')(rl:=RL_tau).
  apply JO_red_ret.
  trivial.
  apply JO_red_star_refl.
 Qed.
 
-Lemma mon_assoc : forall (v v' v'' : value_name) (t t' : typexpr) (a e e' :expr),  
+Lemma mon_assoc : forall (v v' v'' : value_name) (t t' : typexpr) (a e e' :expr)(s s' s'':select),  
     is_value_of_expr a ->
     v <> v'' ->
     v' <> v'' ->
     ((subst_expr a v'' e') = e') ->
     ((subst_expr a v'' e) = e) ->
-    exists (b :expr), (E_live_expr a >>= (E_function v t e) >>= (E_function v' t' e') -->* b) /\ (E_live_expr a >>= (E_function v'' t (E_apply (E_function v t e) (E_ident v'') >>= (E_function v' t' e'))) -->* b).
+    exists (b :expr), (E_live_expr (LM_expr a) >>= (E_function v t e) >>= (E_function v' t' e') -->* b) /\ (E_live_expr (LM_expr a) >>= (E_function v'' t (E_apply (E_function v t e) (E_ident v'') >>= (E_function v' t' e'))) -->* b).
 Proof.
  intros.
  exists (E_apply (E_function v t e) a >>= E_function v' t' e' ).
  split.
  Show 1.
-  apply JO_red_star_step with (e' := ((E_apply (E_function v t e) a) >>= E_function v' t' e')).
+  apply JO_red_star_step with (e' := ((E_apply (E_function v t e) a) >>= E_function v' t' e'))(s:=s)(rl:=RL_tau).
   apply JO_red_evalbind with (e' := ((E_apply (E_function v t e) a))).
   apply JO_red_dobind.
   trivial.
   apply JO_red_star_refl.
- apply JO_red_star_step with (e' := (E_apply (E_function v'' t (E_apply (E_function v t e) (E_ident v'') >>= E_function v' t' e')) a)).
+ apply JO_red_star_step with (e' := (E_apply (E_function v'' t (E_apply (E_function v t e) (E_ident v'') >>= E_function v' t' e')) a))(s:=s')(rl:=RL_tau).
  apply JO_red_dobind.
  trivial.
- apply JO_red_star_step with  (e' := (subst_expr a v'' (E_apply (E_function v t e) (E_ident v'') >>= E_function v' t' e'))).
+ apply JO_red_star_step with  (e' := (subst_expr a v'' (E_apply (E_function v t e) (E_ident v'') >>= E_function v' t' e')))(s:=s'')(rl:=RL_tau).
  apply JO_red_app with (x:=v'') (v:=a) (e := (E_apply (E_function v t e) (E_ident v'') >>= E_function v' t' e')).
  trivial.
  auto.
